README.md
@@ -6,8 +6,4 @@ Atomicity related verification based on Iris logic.
 Build
 --------
 
-1. `git clone` this repo
-2. `git submodule update --init` to fetch corresponding Iris library as a submodule
-3. `cd iris-coq; make; make install` to install Iris library (system globally). Or you can use `make userinstall` to install user globally.
-4. `cd ..; make` to compile this repo
-
+Please make sure Iris dependency version is same as noted in `IRIS_VERSION`
